Equality_Experiments2.v
@@ -1,0 +1,111 @@
+      
+(* 
+  Some experiments with equality.
+  1. About the definitionand the usual properties of equality.
+  2. The Axiom of Extensionality for equality.
+*)
+
+Print eq.
+
+Eval simpl in (eq 2 2).   (* 2=2:Prop *)
+
+Eval simpl in 1=2 /\ 2=2.
+
+(* Coq out-of-the-box example first *)
+
+Lemma coq_equality_is_transitive : forall (T : Type) (x y z: T), 
+ x = y /\ y = z -> x = z.
+Proof. 
+  intros T x y z H. 
+  inversion H as [Hx Hy]. 
+  rewrite -> Hx.
+  rewrite -> Hy.
+  reflexivity.
+Qed.
+
+(* similarly,  = is transitive   *)
+
+Module My_Equality.  (* equality test kitchen *)
+
+(* Print eql. *)   (* not defined *)
+
+Inductive eql {T : Type} (x : T) : T -> Prop :=
+  eql_refl : eql x x.
+
+Print eq.
+Print eql.
+
+Lemma eql_is_transitive_trans : forall (T : Type) (x y z: T), 
+ eql x y /\ eql y z -> eql x z.
+Proof.
+  intros T x y z H.
+  inversion H as [Hx Hy].
+  (* rewrite -> Hx.  NO!  *)
+  induction Hx.
+  induction Hy.
+  (* reflexivity.  NO! *)
+  apply eql_refl.
+Qed.
+
+
+Lemma eql_is_symmetric : forall (T : Type) (x y : T), 
+ eql x y -> eql y x.
+Proof.
+  intros X x y H.  (* i.e. call T X *)
+  induction H.
+  (* reflexivity.  NO! *)
+  apply eql_refl.
+Qed.
+
+
+Lemma eql_is_leibniz_equality : forall (T : Type) (x y: T), 
+ eql x y -> forall P : T -> Prop, P x -> P y.
+Proof.  (* same as for builtin Coq = *)
+intros X x y H.
+induction H.
+intros P H. apply H.
+Qed.
+
+(* eql has same definition as eq so, of course ... *)
+Theorem eql_is_eq : forall (T: Type) (x y : T),
+   eql x y <-> x = y.
+Proof.
+intros T x y. 
+split. 
+(* -> *) 
+intros H. induction H. reflexivity. 
+(* <- *)
+intros H. subst.
+apply eql_refl. 
+Qed.
+
+(* extensionality for our eql *)
+Axiom eql_extensionality : 
+  forall {X Y: Type} {f g : X -> Y},
+    (forall (x: X), f x = g x) ->  eql f g.
+
+Definition f (m : nat) : nat := m+1.
+Definition g (n : nat) : nat := 1+n.
+Definition h (o : nat) : nat := o+1.
+
+Lemma plus_comm : forall n m : nat,
+  n + m = m + n.
+Proof.
+  (* known *) Admitted.
+
+Lemma a : eql f g.
+Proof. apply eql_extensionality.
+(* work from inside out *)
+intros.  unfold f. unfold g. apply plus_comm.
+Qed.
+
+Lemma b : f = h.
+Proof. reflexivity.  (* definitions of f and h unify *)
+Qed.
+
+Lemma c : f = g.
+Proof. (* error reflexivity. *) 
+unfold f. unfold g. (* STUCK  *)
+Abort. (* because = has no extensionality axiom *)
+
+End My_Equality.
